Compartment work

cfrontend/CompartmentSem.v
@@ -56,7 +56,7 @@ Module Type AllocatorAxioms (Ptr: Pointer) (Pol: Policy) (S: Submem Ptr Pol).
 
 End AllocatorAxioms.
 
-Module MemRegionAgnostic (Ptr: Pointer) (Pol: Policy) (Reg: Region) (M: Submem Ptr Pol)
+Module MemRegionAgnostic (Ptr: Pointer) (Pol: Policy) (Reg: Region Ptr) (M: Submem Ptr Pol)
   (A: AllocatorAxioms Ptr Pol M) : Memory Ptr Pol Reg.
 
   Import A.
@@ -160,14 +160,24 @@ Module MemRegionAgnostic (Ptr: Pointer) (Pol: Policy) (Reg: Region) (M: Submem P
 
 End MemRegionAgnostic.
 
-Module CompReg <: Region.
+Module CompReg <: Region SemiconcretePointer.
+  Import SemiconcretePointer.
+
+  Variable bases : block -> int64.
+  
   Inductive region' : Type :=
   | Lcl (CMP: SemiconcretePointer.Comp)
   | Shr (b: block)
   .
 
   Definition region := region'.
-  
+
+  Definition int_to_ptr (i: int64) (r: region) :=
+    match r with
+    | Lcl CMP => P (LocInd CMP) i
+    | Shr b => P (ShareInd b (bases b)) i
+    end.
+                   
 End CompReg.
 
 Module CompartmentCsem (Scheme: CompScheme) (A: AllocatorAxioms SemiconcretePointer NullPolicy M).
@@ -220,180 +230,171 @@ Module CompartmentCsem (Scheme: CompScheme) (A: AllocatorAxioms SemiconcretePoin
     Variable ge: genv.
     Variable ce: composite_env.
 
-  Inductive deref_loc (ty: type) (m: mem) (p: ptr) (pt: val_tag) :
-    bitfield -> trace -> PolicyResult (val * list val_tag * list loc_tag) -> Prop :=
-  | deref_loc_value: forall chunk,
-      access_mode ty = By_value chunk ->
-      type_is_volatile ty = false ->
-      deref_loc ty m p pt Full E0 (load chunk m p)
-  | deref_loc_volatile: forall chunk t res,
-      access_mode ty = By_value chunk -> type_is_volatile ty = true ->
-      volatile_load ge chunk m p t res ->
-      deref_loc ty m p pt Full t res
-  | deref_loc_reference:
+    Inductive deref_loc (ty: type) (m: mem) (p: ptr) (pt: val_tag) :
+      bitfield -> trace -> PolicyResult (val * list val_tag * list loc_tag) -> Prop :=
+    | deref_loc_value: forall chunk,
+        access_mode ty = By_value chunk ->
+        type_is_volatile ty = false ->
+        deref_loc ty m p pt Full E0 (load chunk m p)
+    | deref_loc_volatile: forall chunk t res,
+        access_mode ty = By_value chunk -> type_is_volatile ty = true ->
+        volatile_load ge chunk m p t res ->
+        deref_loc ty m p pt Full t res
+    | deref_loc_reference:
       access_mode ty = By_reference ->
       deref_loc ty m p pt Full E0 (ret (Vptr p, [pt],[]))
-  | deref_loc_copy:
+    | deref_loc_copy:
       access_mode ty = By_copy ->
       deref_loc ty m p pt Full E0 (ret (Vptr p, [pt],[]))
-  | deref_loc_bitfield: forall sz sg pos width res,
-      load_bitfield ty sz sg pos width m p res ->
-      deref_loc ty m p pt (Bits sz sg pos width) E0 res.
+    | deref_loc_bitfield: forall sz sg pos width res,
+        load_bitfield ty sz sg pos width m p res ->
+        deref_loc ty m p pt (Bits sz sg pos width) E0 res.
 
-  Inductive assign_loc (ty: type) (m: mem) (p: ptr) (pt: val_tag) (lts: list loc_tag):
-    bitfield -> atom -> trace -> PolicyResult (mem * atom) -> Prop :=
-  | assign_loc_value: forall v vt chunk res,
-      access_mode ty = By_value chunk ->
-      type_is_volatile ty = false ->
-      res = m' <- store chunk m p (v,vt) lts;;
-            ret (m',(v,vt)) ->
-      assign_loc ty m p pt lts Full (v,vt) E0 res
-  | assign_loc_volatile: forall v chunk t res res',
-      access_mode ty = By_value chunk -> type_is_volatile ty = true ->
-      volatile_store ge chunk m p v lts t res ->
-      res' = m' <- res;; ret (m',v) ->
-      assign_loc ty m p pt lts Full v t res'
-  | assign_loc_copy: forall p_src pt' res,
-      access_mode ty = By_copy ->
-      (alignof_blockcopy ce ty = alignp p_src) ->
-      (alignof_blockcopy ce ty = alignp p (*dst*)) ->
-      p_src = p (*dst*)
-      \/ le (off p_src (Int64.repr (sizeof ce ty))) p (*dst*)
-      \/ le (off p (*dst*) (Int64.repr (sizeof ce ty))) p_src ->
-      res = bytes <- loadbytes m p_src (sizeof ce ty);;
-            m' <- storebytes m p (*dst*) bytes lts;;
-            ret (m', (Vptr p (*dst*), pt')) ->
-      assign_loc ty m p (*dst*) pt lts Full (Vptr p_src, pt') E0 res
-  | assign_loc_bitfield: forall sz sg pos width v res,
-      store_bitfield ty sz sg pos width m p pt v lts res ->
-      assign_loc ty m p pt lts (Bits sz sg pos width) v E0 res.
- 
+    Inductive assign_loc (ty: type) (m: mem) (p: ptr) (pt: val_tag) (lts: list loc_tag):
+      bitfield -> atom -> trace -> PolicyResult (mem * atom) -> Prop :=
+    | assign_loc_value: forall v vt chunk res,
+        access_mode ty = By_value chunk ->
+        type_is_volatile ty = false ->
+        res = m' <- store chunk m p (v,vt) lts;;
+              ret (m',(v,vt)) ->
+        assign_loc ty m p pt lts Full (v,vt) E0 res
+    | assign_loc_volatile: forall v chunk t res res',
+        access_mode ty = By_value chunk -> type_is_volatile ty = true ->
+        volatile_store ge chunk m p v lts t res ->
+        res' = m' <- res;; ret (m',v) ->
+        assign_loc ty m p pt lts Full v t res'
+    | assign_loc_copy: forall p_src pt' res,
+        access_mode ty = By_copy ->
+        (alignof_blockcopy ce ty = alignp p_src) ->
+        (alignof_blockcopy ce ty = alignp p (*dst*)) ->
+        p_src = p (*dst*)
+        \/ le (off p_src (Int64.repr (sizeof ce ty))) p (*dst*)
+        \/ le (off p (*dst*) (Int64.repr (sizeof ce ty))) p_src ->
+        res = bytes <- loadbytes m p_src (sizeof ce ty);;
+              m' <- storebytes m p (*dst*) bytes lts;;
+              ret (m', (Vptr p (*dst*), pt')) ->
+        assign_loc ty m p (*dst*) pt lts Full (Vptr p_src, pt') E0 res
+    | assign_loc_bitfield: forall sz sg pos width v res,
+        store_bitfield ty sz sg pos width m p pt v lts res ->
+        assign_loc ty m p pt lts (Bits sz sg pos width) v E0 res.
     
-  Fixpoint chunk_of_type (ty:type) :=
-    match ty with
-    | Tint sz sgn _ =>
-        match sz, sgn with
-        | I8, Signed | IBool, Signed => Mint8signed
-        | I8, Unsigned | IBool, Unsigned => Mint8unsigned
-        | I16, Signed => Mint8signed
-        | I16, Unsigned => Mint8unsigned
-        | I32, _ => Mint32
-        end
-    | Tlong _ _ => Mint64
-    | Tfloat F32 _ => Mfloat32
-    | Tfloat F64 _ => Mfloat64
-    | Tarray ty' _ _ => chunk_of_type ty'
-    | _ => Mint64 (* composite types are pointers are longs *)
-    end.
-
-  (* Allocates local (public) variables *)
-  Definition do_alloc_variable (l: Cabs.loc) (CMP: Comp) (bg: block_generator) (e: env) (m: mem) (id: ident) (ty:type) (shared: bool):
-    PolicyResult (block_generator * env * mem) :=
-    '(m',base) <- stkalloc m (Lcl CMP) (alignof ce ty) (sizeof ce ty);;
-    ret (bg, PTree.set id (PUB base tt ty) e, m').
-
-  Definition do_alloc_variables (l: Cabs.loc) (CMP: Comp) (bg: block_generator) (e: env) (m: mem) (vs: list (ident * type)) (shared: bool) :
-    PolicyResult (block_generator * env * mem) :=
-    fold_left (fun res '(id,ty) =>
-                 '(bg', e',m') <- res;;
-                 do_alloc_variable l CMP bg e' m' id ty shared)
-              vs (ret (bg, e, m)).
-
-  (* Allocates local (public) arguments and initializes them with their corresponding values *)
-  Definition do_init_param (l: Cabs.loc) (CMP: Comp) (bg: block_generator) (e: env) (m: mem) (id: ident) (ty: type) (init: option atom) :
-    PolicyResult (block_generator * env * mem) :=
-    '(bg', e', m') <- do_alloc_variable l CMP bg e m id ty false;;
-    match e'!id, init with
-    | Some (PUB base _ _), Some init =>
-        m'' <- store_atom (chunk_of_type ty) m' base init;;
-        ret (bg', e',m'')
-    | _, _ => ret (bg', e', m')
-    end.
-
-  Definition do_init_params (l: Cabs.loc) (CMP: Comp) (bg: block_generator) (e: env) (m: mem)
-             (ps: list (ident * type * option atom))
-    : PolicyResult (block_generator * env * mem) :=
-    fold_left (fun res '(id,ty,init) =>
-                 '(bg', e',m') <- res;;
-                 do_init_param l CMP bg e' m' id ty init)
-              ps (ret (bg, e, m)).    
     
-  Fixpoint do_free_variables (l: Cabs.loc) (CMP: Comp) (pct: control_tag) (m: mem) (vs: list (ptr*type))
-    : PolicyResult (control_tag * mem) :=
-    match vs with
-    | [] => ret (pct,m)
-    | (base,ty) :: vs' =>
-        m' <- stkfree m (Lcl CMP) (alignof ce ty) (sizeof ce ty);;
-        '(pct', vt', lts') <- DeallocT l ce pct ty;;
-        do_free_variables l CMP pct' m' vs'
-    end.
+    Fixpoint chunk_of_type (ty:type) :=
+      match ty with
+      | Tint sz sgn _ =>
+          match sz, sgn with
+          | I8, Signed | IBool, Signed => Mint8signed
+          | I8, Unsigned | IBool, Unsigned => Mint8unsigned
+          | I16, Signed => Mint8signed
+          | I16, Unsigned => Mint8unsigned
+          | I32, _ => Mint32
+          end
+      | Tlong _ _ => Mint64
+      | Tfloat F32 _ => Mfloat32
+      | Tfloat F64 _ => Mfloat64
+      | Tarray ty' _ _ => chunk_of_type ty'
+      | _ => Mint64 (* composite types are pointers are longs *)
+      end.
 
-  (** Return the list of types in the (public) codomain of [e]. *)
-  Definition variables_of_env (e: env) : list (ptr*type) :=
-    List.fold_left (fun acc '(_,entry) =>
-                      match entry with
-                      | PUB base pt ty =>
-                          (base,ty)::acc
-                      | PRIV ty => acc
-                      end) (PTree.elements e) [].
+    (* Allocates local (public) variables *)
+    Definition do_alloc_variable (l: Cabs.loc) (CMP: Comp) (bg: block_generator) (e: env) (m: mem) (id: ident) (ty:type) (shared: bool):
+      PolicyResult (block_generator * env * mem) :=
+      '(m',base) <- stkalloc m (Lcl CMP) (alignof ce ty) (sizeof ce ty);;
+      ret (bg, PTree.set id (PUB base tt ty) e, m').
+
+    Definition do_alloc_variables (l: Cabs.loc) (CMP: Comp) (bg: block_generator) (e: env) (m: mem) (vs: list (ident * type)) (shared: bool) :
+      PolicyResult (block_generator * env * mem) :=
+      fold_left (fun res '(id,ty) =>
+                   '(bg', e',m') <- res;;
+                   do_alloc_variable l CMP bg e' m' id ty shared)
+                vs (ret (bg, e, m)).
+
+    (* Allocates local (public) arguments and initializes them with their corresponding values *)
+    Definition do_init_param (l: Cabs.loc) (CMP: Comp) (bg: block_generator) (e: env) (m: mem) (id: ident) (ty: type) (init: option atom) :
+      PolicyResult (block_generator * env * mem) :=
+      '(bg', e', m') <- do_alloc_variable l CMP bg e m id ty false;;
+      match e'!id, init with
+      | Some (PUB base _ _), Some init =>
+          m'' <- store_atom (chunk_of_type ty) m' base init;;
+          ret (bg', e',m'')
+      | _, _ => ret (bg', e', m')
+      end.
+
+    Definition do_init_params (l: Cabs.loc) (CMP: Comp) (bg: block_generator) (e: env) (m: mem)
+               (ps: list (ident * type * option atom))
+      : PolicyResult (block_generator * env * mem) :=
+      fold_left (fun res '(id,ty,init) =>
+                   '(bg', e',m') <- res;;
+                   do_init_param l CMP bg e' m' id ty init)
+                ps (ret (bg, e, m)).    
+    
+    Fixpoint do_free_variables (l: Cabs.loc) (CMP: Comp) (pct: control_tag) (m: mem) (vs: list (ptr*type))
+      : PolicyResult (control_tag * mem) :=
+      match vs with
+      | [] => ret (pct,m)
+      | (base,ty) :: vs' =>
+          m' <- stkfree m (Lcl CMP) (alignof ce ty) (sizeof ce ty);;
+          '(pct', vt', lts') <- DeallocT l ce pct ty;;
+          do_free_variables l CMP pct' m' vs'
+      end.
+
+    (** Return the list of types in the (public) codomain of [e]. *)
+    Definition variables_of_env (e: env) : list (ptr*type) :=
+      List.fold_left (fun acc '(_,entry) =>
+                        match entry with
+                        | PUB base pt ty =>
+                            (base,ty)::acc
+                        | PRIV ty => acc
+                        end) (PTree.elements e) [].
 
     (** Selection of the appropriate case of a [switch], given the value [n]
-      of the selector expression. *)
+        of the selector expression. *)
 
-  Fixpoint select_switch_default (sl: labeled_statements): labeled_statements :=
-    match sl with
-    | LSnil => sl
-    | LScons None s sl' => sl
-    | LScons (Some i) s sl' => select_switch_default sl'
-    end.
+    Fixpoint select_switch_default (sl: labeled_statements): labeled_statements :=
+      match sl with
+      | LSnil => sl
+      | LScons None s sl' => sl
+      | LScons (Some i) s sl' => select_switch_default sl'
+      end.
 
-  Fixpoint select_switch_case (n: Z) (sl: labeled_statements): option labeled_statements :=
-    match sl with
-    | LSnil => None
-    | LScons None s sl' => select_switch_case n sl'
-    | LScons (Some c) s sl' => if zeq c n then Some sl else select_switch_case n sl'
-    end.
+    Fixpoint select_switch_case (n: Z) (sl: labeled_statements): option labeled_statements :=
+      match sl with
+      | LSnil => None
+      | LScons None s sl' => select_switch_case n sl'
+      | LScons (Some c) s sl' => if zeq c n then Some sl else select_switch_case n sl'
+      end.
 
-  Definition select_switch (n: Z) (sl: labeled_statements): labeled_statements :=
-    match select_switch_case n sl with
-    | Some sl' => sl'
-    | None => select_switch_default sl
-    end.
+    Definition select_switch (n: Z) (sl: labeled_statements): labeled_statements :=
+      match select_switch_case n sl with
+      | Some sl' => sl'
+      | None => select_switch_default sl
+      end.
 
-  (** Turn a labeled statement into a sequence *)
+    (** Turn a labeled statement into a sequence *)
 
-  Fixpoint seq_of_labeled_statement (sl: labeled_statements) : statement :=
-    match sl with
-    | LSnil => Sskip
-    | LScons _ s sl' => Ssequence s (seq_of_labeled_statement sl')
-    end.
+    Fixpoint seq_of_labeled_statement (sl: labeled_statements) : statement :=
+      match sl with
+      | LSnil => Sskip
+      | LScons _ s sl' => Ssequence s (seq_of_labeled_statement sl')
+      end.
 
-  Fixpoint exprlist_len (el:exprlist) : nat :=
-    match el with
-    | Enil => O
-    | Econs _ el' => (exprlist_len el')+1
-    end.
+    Fixpoint exprlist_len (el:exprlist) : nat :=
+      match el with
+      | Enil => O
+      | Econs _ el' => (exprlist_len el')+1
+      end.
    
     (** Extract the values from a list of function arguments *)
-  Inductive cast_arguments (l:Cabs.loc) (pct: control_tag) (fpt: val_tag) (m: mem):
-    exprlist -> typelist -> PolicyResult (control_tag * list atom) -> Prop :=
-  | cast_args_nil:
-    cast_arguments l pct fpt m Enil Tnil (ret (pct, []))
-  | cast_args_cons: forall pct' pct'' v vt vt' ty el targ1 targs v1 vl,
-      sem_cast v ty targ1 m = Some v1 ->
-      cast_arguments l pct' fpt m el targs (ret (pct'',vl)) ->
-      cast_arguments l pct fpt m (Econs (Eval (v,vt) ty) el) (Tcons targ1 targs)
-                     (ret (pct'',(v1, vt') :: vl))
-  | cast_args_fail_now: forall v v1 vt ty el targ1 targs failure,
-      sem_cast v ty targ1 m = Some v1 ->
-      cast_arguments l pct fpt m (Econs (Eval (v,vt) ty) el) (Tcons targ1 targs)
-                     (raise failure)
-  | cast_args_fail_later: forall pct' v vt ty el targ1 targs v1 failure,
-      sem_cast v ty targ1 m = Some v1 ->
-      cast_arguments l pct' fpt m el targs (raise failure) ->
-      cast_arguments l pct fpt m (Econs (Eval (v,vt) ty) el) (Tcons targ1 targs)
-                     (raise failure)
-  .
+    Inductive cast_arguments (l:Cabs.loc) (CMP: Comp) (fpt: val_tag) (m: mem):
+      exprlist -> typelist -> PolicyResult (list atom) -> Prop :=
+    | cast_args_nil:
+      cast_arguments l CMP fpt m Enil Tnil (ret [])
+    | cast_args_cons: forall v vt ty el targ1 targs v1 vl,
+        sem_cast v ty targ1 (Lcl CMP) = Some v1 ->
+        cast_arguments l CMP fpt m el targs (ret vl) ->
+        cast_arguments l CMP fpt m (Econs (Eval (v,vt) ty) el) (Tcons targ1 targs)
+                       (ret ((v1, tt) :: vl))
+    .
   
     (** ** Reduction semantics for expressions *)
 
@@ -408,448 +409,285 @@ Module CompartmentCsem (Scheme: CompScheme) (A: AllocatorAxioms SemiconcretePoin
       (bind_prop_success_rel P A PS1 PS2)
         (at level 62, right associativity, A pattern).
 
-
   Section EXPR.
 
     Variable e: env.
     Variable l: Cabs.loc.
+    Variable CMP: Comp.
      
-    Inductive lred : expr -> control_tag -> tenv -> mem ->
+    Inductive lred : expr -> tenv -> mem ->
                      expr -> tenv -> mem ->
                      pstate -> pstate -> Prop :=
-    | red_var_tmp: forall x ty pct te m ps,
+    | red_var_tmp: forall x ty te m ps,
         e!x = Some (PRIV ty) ->
-        lred (Evar x ty) pct te m
+        lred (Evar x ty) te m
              (Eloc (Ltmp x) ty) te m ps ps
-    | red_var_local: forall x pt ty pct base te m ps,
+    | red_var_local: forall x pt ty base te m ps,
         e!x = Some (PUB base pt ty) ->
-        lred (Evar x ty) pct te m
+        lred (Evar x ty) te m
              (Eloc (Lmem base pt Full) ty) te m ps ps
-    | red_var_global: forall x ty pct base bound pt gv te m ps,
+    | red_var_global: forall x ty base bound pt gv te m ps,
         e!x = None ->
         Genv.find_symbol ge x = Some (SymGlob base bound pt gv) ->
-        lred (Evar x ty) pct te m
+        lred (Evar x ty) te m
              (Eloc (Lmem base pt Full) ty) te m ps ps
-    | red_func: forall x pct b pt ty te m ps,
+    | red_func: forall x b pt ty te m ps,
         e!x = None ->
         Genv.find_symbol ge x = Some (SymIFun _ b pt) ->
-        lred (Evar x ty) pct te m
+        lred (Evar x ty) te m
              (Eloc (Lifun b pt) ty) te m ps ps
-    | red_ext_func: forall x pct ef tyargs tyres cc pt ty te m ps,
+    | red_ext_func: forall x ef tyargs tyres cc pt ty te m ps,
         e!x = None ->
         Genv.find_symbol ge x = Some (SymEFun _ ef tyargs tyres cc pt) ->
-        lred (Evar x ty) pct te m
+        lred (Evar x ty) te m
              (Eloc (Lefun ef tyargs tyres cc pt) ty) te m ps ps
-    | red_builtin: forall ef tyargs cc ty pct te m ps,
-        lred (Ebuiltin ef tyargs cc ty) pct te m
+    | red_builtin: forall ef tyargs cc ty te m ps,
+        lred (Ebuiltin ef tyargs cc ty) te m
              (Eloc (Lefun ef tyargs Tany64 cc def_tag) ty) te m ps ps
-    | red_deref: forall p vt ty1 ty pct te m ps,
-        lred (Ederef (Eval (Vptr p,vt) ty1) ty) pct te m
+    | red_deref: forall p vt ty1 ty te m ps,
+        lred (Ederef (Eval (Vptr p,vt) ty1) ty) te m
              (Eloc (Lmem p vt Full) ty) te m ps ps
-    | red_field_struct: forall p pt pt' id co a f ty pct delta bf te m ps0 ps1,
+    | red_field_struct: forall p pt pt' id co a f ty delta bf te m ps0 ps1,
         ce!id = Some co ->
         field_offset ce f (co_members co) = OK (delta, bf) ->
-        FieldT l ce pct pt ty id ps0 = (Success pt',ps1) ->
-        lred (Efield (Eval (Vptr p, pt) (Tstruct id a)) f ty) pct te m
+        lred (Efield (Eval (Vptr p, pt) (Tstruct id a)) f ty) te m
              (Eloc (Lmem (off p (Int64.repr delta)) pt' bf) ty) te m ps0 ps1
-    | red_field_union: forall p pt pt' id co a f ty pct delta bf te m ps0 ps1,
+    | red_field_union: forall p pt pt' id co a f ty delta bf te m ps0 ps1,
         ce!id = Some co ->
         union_field_offset ce f (co_members co) = OK (delta, bf) ->
-        FieldT l ce pct pt ty id ps0 = (Success pt',ps1) ->
-        lred (Efield (Eval (Vptr p, pt) (Tunion id a)) f ty) pct te m
+        lred (Efield (Eval (Vptr p, pt) (Tunion id a)) f ty) te m
              (Eloc (Lmem (off p (Int64.repr delta)) pt' bf) ty) te m ps0 ps1.
 
     (** Head reductions for r-values *)
-    Inductive rred (pct:control_tag) :
-      expr -> tenv -> mem -> trace -> control_tag ->
+    Inductive rred :
+      expr -> tenv -> mem -> trace ->
       expr -> tenv -> mem -> pstate -> pstate -> Prop :=
     | red_const: forall v ty te m vt' ps0 ps1,
-        ConstT l pct ps0 = (Success vt',ps1) ->
-        rred pct (Econst v ty) te m E0 pct (Eval (v,vt') ty) te m ps0 ps1
+        rred (Econst v ty) te m E0 (Eval (v,vt') ty) te m ps0 ps1
     | red_rvalof_mem: forall ofs pt lts bf ty te m tr v vts vt'' ps0 ps1 ps2,
         deref_loc ty m ofs pt bf tr <<ps0>> (Success (v, vts, lts)) <<ps1>> ->
-        (vt <- CoalesceT l vts;;
-         vt' <- LoadT l pct pt vt lts;;
-         AccessT l pct vt') ps1 = (Success vt'',ps2) ->
-        rred pct (Evalof (Eloc (Lmem ofs pt bf) ty) ty) te m tr
-             pct (Eval (v,vt'') ty) te m ps0 ps2
+        rred (Evalof (Eloc (Lmem ofs pt bf) ty) ty) te m tr
+             (Eval (v,vt'') ty) te m ps0 ps2
     | red_rvalof_ifun: forall b pt ty te m ps,
-        rred pct (Evalof (Eloc (Lifun b pt) ty) ty) te m E0
-             pct (Eval (Vfptr b, pt) ty) te m ps ps
+        rred (Evalof (Eloc (Lifun b pt) ty) ty) te m E0
+             (Eval (Vfptr b, pt) ty) te m ps ps
     | red_rvalof_efun: forall ef tyargs tyres cc pt ty te m ps,
-        rred pct (Evalof (Eloc (Lefun ef tyargs tyres cc pt) ty) ty) te m E0
-             pct (Eval (Vefptr ef tyargs tyres cc, pt) ty) te m ps ps
+        rred (Evalof (Eloc (Lefun ef tyargs tyres cc pt) ty) ty) te m E0
+             (Eval (Vefptr ef tyargs tyres cc, pt) ty) te m ps ps
     | red_rvalof_tmp: forall b ty te m v vt vt' ps0 ps1,
         te!b = Some (v,vt) ->
-        AccessT l pct vt ps0 = (Success vt',ps1) ->
-        rred pct (Evalof (Eloc (Ltmp b) ty) ty) te m E0
-             pct (Eval (v,vt') ty) te m ps0 ps1
+        rred (Evalof (Eloc (Ltmp b) ty) ty) te m E0
+             (Eval (v,vt') ty) te m ps0 ps1
     | red_addrof_loc: forall ofs pt ty1 ty te m ps,
-        rred pct (Eaddrof (Eloc (Lmem ofs pt Full) ty1) ty) te m E0
-             pct (Eval (Vptr ofs, pt) ty) te m ps ps
+        rred (Eaddrof (Eloc (Lmem ofs pt Full) ty1) ty) te m E0
+             (Eval (Vptr ofs, pt) ty) te m ps ps
     | red_addrof_fptr: forall b pt ty te m ps,
-        rred pct (Eaddrof (Eloc (Lifun b pt) ty) ty) te m E0
-             pct (Eval (Vfptr b, pt) ty) te m ps ps
+        rred (Eaddrof (Eloc (Lifun b pt) ty) ty) te m E0
+             (Eval (Vfptr b, pt) ty) te m ps ps
     | red_addrof_efptr: forall ef tyargs tyres cc pt ty te m ps,
-        rred pct (Eaddrof (Eloc (Lefun ef tyargs tyres cc pt) ty) ty) te m E0
-             pct (Eval (Vefptr ef tyargs tyres cc, pt) ty) te m ps ps
-    | red_unop: forall op v1 vt1 ty1 ty te m v pct' vt ps0 ps1,
+        rred (Eaddrof (Eloc (Lefun ef tyargs tyres cc pt) ty) ty) te m E0
+             (Eval (Vefptr ef tyargs tyres cc, pt) ty) te m ps ps
+    | red_unop: forall op v1 vt1 ty1 ty te m v vt ps0 ps1,
         sem_unary_operation op v1 ty1 m = Some v ->
-        UnopT l op pct vt1 ps0 = (Success (pct', vt), ps1) ->
-        rred pct (Eunop op (Eval (v1,vt1) ty1) ty) te m E0
-             pct' (Eval (v,vt) ty) te m ps0 ps1
-    | red_binop: forall op v1 vt1 ty1 v2 vt2 ty2 ty te m v vt' pct' ps0 ps1,
-        sem_binary_operation ce op v1 ty1 v2 ty2 m = Some v ->
-        BinopT l op pct vt1 vt2 ps0 = (Success (pct', vt'), ps1) ->
-        rred pct (Ebinop op (Eval (v1,vt1) ty1) (Eval (v2,vt2) ty2) ty) te m E0
-             pct' (Eval (v,vt') ty) te m ps0 ps1
+        rred (Eunop op (Eval (v1,vt1) ty1) ty) te m E0
+             (Eval (v,vt) ty) te m ps0 ps1
+    | red_binop: forall op v1 vt1 ty1 v2 vt2 ty2 ty te m v vt' ps0 ps1,
+        sem_binary_operation ce op v1 ty1 v2 ty2 (Lcl CMP) = Some v ->
+        rred (Ebinop op (Eval (v1,vt1) ty1) (Eval (v2,vt2) ty2) ty) te m E0
+             (Eval (v,vt') ty) te m ps0 ps1
     | red_cast_int_int: forall ty v1 vt1 ty1 te m v vt' ps0 ps1,
         (forall ty' attr, ty1 <> Tpointer ty' attr) ->
         (forall ty' attr, ty <> Tpointer ty' attr) ->
-        sem_cast v1 ty1 ty m = Some v ->
-        IICastT l pct vt1 ty ps0 = (Success vt',ps1) -> 
-        rred pct (Ecast (Eval (v1,vt1) ty1) ty) te m E0
-             pct (Eval (v,vt') ty) te m ps0 ps1
+        sem_cast v1 ty1 ty (Lcl CMP) = Some v ->
+        rred (Ecast (Eval (v1,vt1) ty1) ty) te m E0
+             (Eval (v,vt') ty) te m ps0 ps1
     | red_cast_int_ptr: forall ty v1 vt1 ty1 te m v ofs tr v2 vt2 lts pt' ty' attr ps0 ps1 ps2,
         (forall ty' attr, ty1 <> Tpointer ty' attr) ->
         ty = Tpointer ty' attr ->
-        sem_cast v1 ty1 ty m = Some v ->
+        sem_cast v1 ty1 ty (Lcl CMP) = Some v ->
         v = Vptr ofs ->
         deref_loc ty m ofs vt1 Full tr <<ps0>> (Success ((v2,vt2), lts)) <<ps1>> ->
-        IPCastT l pct vt1 (Some lts) ty ps1 = (Success pt', ps2) ->
-        rred pct (Ecast (Eval (v1,vt1) ty1) ty) te m tr
-             pct (Eval (v,pt') ty) te m ps0 ps2
+        rred (Ecast (Eval (v1,vt1) ty1) ty) te m tr
+             (Eval (v,pt') ty) te m ps0 ps2
     | red_cast_ptr_int: forall ty v1 vt1 ty1 te m v ofs tr v2 vt2 lts vt' ty' attr ps0 ps1 ps2,
         ty1 = Tpointer ty' attr ->
         (forall ty' attr, ty <> Tpointer ty' attr) ->
-        sem_cast v1 ty1 ty m = Some v ->
+        sem_cast v1 ty1 ty (Lcl CMP) = Some v ->
         v1 = Vptr ofs ->
         deref_loc ty1 m ofs vt1 Full tr <<ps0>> (Success ((v2,vt2), lts)) <<ps1>> ->
-        PICastT l pct vt1 (Some lts) ty ps1 = (Success vt',ps2) ->
-        rred pct (Ecast (Eval (v1,vt1) ty1) ty) te m tr
-             pct (Eval (v,vt') ty) te m ps0 ps2
+        rred (Ecast (Eval (v1,vt1) ty1) ty) te m tr
+             (Eval (v,vt') ty) te m ps0 ps2
     | red_cast_ptr_ptr: forall ty v1 vt1 ty1 te m v ofs ofs1 tr tr1
                                v2 vt2 v3 vt3 lts lts1 ty1' attr1 ty' attr2 pt' ps0 ps1 ps2 ps3,
         ty1 = Tpointer ty1' attr1 ->
         ty = Tpointer ty' attr2 ->
-        sem_cast v1 ty1 ty m = Some v ->
+        sem_cast v1 ty1 ty (Lcl CMP) = Some v ->
         v1 = Vptr ofs1 -> v = Vptr ofs ->
         deref_loc ty1 m ofs1 vt1 Full tr1 <<ps0>> (Success ((v2,vt2),lts1)) <<ps1>> ->
         deref_loc ty m ofs vt1 Full tr <<ps1>> (Success ((v3,vt3),lts)) <<ps2>> ->
-        PPCastT l pct vt1 (Some lts1) (Some lts) ty ps2 = (Success pt',ps3) ->
-        rred pct (Ecast (Eval (v1,vt1) ty1) ty) te m (tr1 ++ tr)
-             pct (Eval (v,pt') ty) te m ps0 ps3
-    | red_seqand_true: forall v1 vt1 ty1 r2 ty te m pct' ps0 ps1,
+        rred (Ecast (Eval (v1,vt1) ty1) ty) te m (tr1 ++ tr)
+             (Eval (v,pt') ty) te m ps0 ps3
+    | red_seqand_true: forall v1 vt1 ty1 r2 ty te m ps0 ps1,
         bool_val v1 ty1 m = Some true ->
-        ExprSplitT l pct vt1 ps0 = (Success pct',ps1) ->
-        rred pct (Eseqand (Eval (v1,vt1) ty1) r2 ty) te m E0
-             pct' (Eparen r2 type_bool ty) te m ps0 ps1
-    | red_seqand_false: forall v1 vt1 ty1 r2 ty te m pct' ps0 ps1,
+        rred (Eseqand (Eval (v1,vt1) ty1) r2 ty) te m E0
+             (Eparen r2 type_bool ty) te m ps0 ps1
+    | red_seqand_false: forall v1 vt1 ty1 r2 ty te m ps0 ps1,
         bool_val v1 ty1 m = Some false ->
-        ExprSplitT l pct vt1 ps0 = (Success pct',ps1) ->
-        rred pct (Eseqand (Eval (v1,vt1) ty1) r2 ty) te m E0
-             pct' (Eval (Vint Int.zero, vt1) ty) te m ps0 ps1
-    | red_seqor_true: forall v1 vt1 ty1 r2 ty te m pct' ps0 ps1,
+        rred (Eseqand (Eval (v1,vt1) ty1) r2 ty) te m E0
+             (Eval (Vint Int.zero, vt1) ty) te m ps0 ps1
+    | red_seqor_true: forall v1 vt1 ty1 r2 ty te m ps0 ps1,
         bool_val v1 ty1 m = Some true ->
-        ExprSplitT l pct vt1 ps0 = (Success pct', ps1) ->
-        rred pct (Eseqor (Eval (v1,vt1) ty1) r2 ty) te m E0
-             pct' (Eval (Vint Int.one, vt1) ty) te m ps0 ps1
-    | red_seqor_false: forall v1 vt1 ty1 r2 ty te m pct' ps0 ps1,
+        rred (Eseqor (Eval (v1,vt1) ty1) r2 ty) te m E0
+             (Eval (Vint Int.one, vt1) ty) te m ps0 ps1
+    | red_seqor_false: forall v1 vt1 ty1 r2 ty te m ps0 ps1,
         bool_val v1 ty1 m = Some false ->
-        ExprSplitT l pct vt1 ps0 = (Success pct',ps1) ->
-        rred pct (Eseqor (Eval (v1,vt1) ty1) r2 ty) te m E0
-             pct' (Eparen r2 type_bool ty) te m ps0 ps1
-    | red_condition: forall v1 vt1 ty1 r1 r2 ty b te m pct' ps0 ps1,
+        rred (Eseqor (Eval (v1,vt1) ty1) r2 ty) te m E0
+             (Eparen r2 type_bool ty) te m ps0 ps1
+    | red_condition: forall v1 vt1 ty1 r1 r2 ty b te m ps0 ps1,
         bool_val v1 ty1 m = Some b ->
-        ExprSplitT l pct vt1 ps0 = (Success pct',ps1) ->
-        rred pct (Econdition (Eval (v1,vt1) ty1) r1 r2 ty) te m E0
-             pct' (Eparen (if b then r1 else r2) ty ty) te m ps0 ps1
+        rred (Econdition (Eval (v1,vt1) ty1) r1 r2 ty) te m E0
+             (Eparen (if b then r1 else r2) ty ty) te m ps0 ps1
     | red_sizeof: forall ty1 ty te m vt' ps0 ps1,
-        ConstT l pct ps0 = (Success vt',ps1) ->
-        rred pct (Esizeof ty1 ty) te m E0
-             pct (Eval (Vlong (Int64.repr (sizeof ce ty1)), vt') ty) te m ps0 ps1
+        rred (Esizeof ty1 ty) te m E0
+             (Eval (Vlong (Int64.repr (sizeof ce ty1)), vt') ty) te m ps0 ps1
     | red_alignof: forall ty1 ty te m vt' ps0 ps1,
-        ConstT l pct ps0 = (Success vt',ps1) ->
-        rred pct (Ealignof ty1 ty) te m E0
-        pct (Eval (Vlong (Int64.repr (alignof ce ty1)), vt') ty) te m ps0 ps1
+        rred (Ealignof ty1 ty) te m E0
+             (Eval (Vlong (Int64.repr (alignof ce ty1)), vt') ty) te m ps0 ps1
     | red_assign_mem: forall ofs ty1 pt bf v1 vts v2 vt2 ty2 te m t1 t2 m' v'
-                             pct'' vt'' v'' vt''' lts lts' ps0 ps1 ps2 ps3,
-        sem_cast v2 ty2 ty1 m = Some v' ->
+                             vt'' v'' vt''' lts lts' ps0 ps1 ps2 ps3,
+        sem_cast v2 ty2 ty1 (Lcl CMP) = Some v' ->
         deref_loc ty1 m ofs pt bf t1 <<ps0>> (Success (v1, vts, lts)) <<ps1>> ->
-        ('(pct',vt') <- AssignT l pct (EffectiveT l vts) vt2;;
-        StoreT l pct' pt vt' lts) ps1 = (Success (pct'', vt'', lts'),ps2) ->
         assign_loc ty1 m ofs pt lts' bf (v',vt'') t2 <<ps2>> (Success (m', (v'',vt'''))) <<ps3>> ->
-        rred pct (Eassign (Eloc (Lmem ofs pt bf) ty1) (Eval (v2, vt2) ty2) ty1) te m (t1++t2)
-             pct'' (Eval (v'',vt''') ty1) te m' ps0 ps3
-    | red_assign_tmp: forall b ty1 v1 vt1 v2 vt2 ty2 te m te' v pct' vt' ps0 ps1,
+        rred (Eassign (Eloc (Lmem ofs pt bf) ty1) (Eval (v2, vt2) ty2) ty1) te m (t1++t2)
+             (Eval (v'',vt''') ty1) te m' ps0 ps3
+    | red_assign_tmp: forall b ty1 v1 vt1 v2 vt2 ty2 te m te' v vt' ps0 ps1,
         te!b = Some (v1,vt1) ->
-        sem_cast v2 ty2 ty1 m = Some v ->
+        sem_cast v2 ty2 ty1 (Lcl CMP) = Some v ->
         te' = PTree.set b (v,vt') te ->
-        AssignT l pct vt1 vt2 ps0 = (Success (pct',vt'),ps1) ->
-        rred pct (Eassign (Eloc (Ltmp b) ty1) (Eval (v2, vt2) ty2) ty1) te m E0
-             pct' (Eval (v,vt') ty1) te' m ps0 ps1
+        rred (Eassign (Eloc (Ltmp b) ty1) (Eval (v2, vt2) ty2) ty1) te m E0
+             (Eval (v,vt') ty1) te' m ps0 ps1
     | red_assignop_mem: forall op ofs pt ty1 bf v2 vt2 ty2 tyres te m t
                                v1 vts vt1'' lts ps0 ps1 ps2,
         deref_loc ty1 m ofs pt bf t <<ps0>> (Success (v1, vts, lts)) <<ps1>> ->
-        (vt1 <- CoalesceT l vts;;
-         vt1' <- LoadT l pct pt vt1 lts;;
-         AccessT l pct vt1') ps1 = (Success vt1'',ps2) ->
-        rred pct (Eassignop op (Eloc (Lmem ofs pt bf) ty1) (Eval (v2,vt2) ty2) tyres ty1) te m t
-             pct (Eassign (Eloc (Lmem ofs pt bf) ty1)
-                          (Ebinop op (Eval (v1,vt1'') ty1) (Eval (v2,vt2) ty2) tyres) ty1) te m ps0 ps2
+        rred (Eassignop op (Eloc (Lmem ofs pt bf) ty1) (Eval (v2,vt2) ty2) tyres ty1) te m t
+             (Eassign (Eloc (Lmem ofs pt bf) ty1)
+                      (Ebinop op (Eval (v1,vt1'') ty1) (Eval (v2,vt2) ty2) tyres) ty1) te m ps0 ps2
     | red_assignop_tmp: forall op b ty1 v2 vt2 ty2 tyres te m v1 vt1 vt1' ps0 ps1,
         te!b = Some (v1,vt1) ->
-        AccessT l pct vt1 ps0 = (Success vt1',ps1) ->
-        rred pct (Eassignop op (Eloc (Ltmp b) ty1) (Eval (v2,vt2) ty2) tyres ty1) te m E0
-             pct (Eassign (Eloc (Ltmp b) ty1)
-                          (Ebinop op (Eval (v1,vt1') ty1) (Eval (v2,vt2) ty2) tyres) ty1) te m ps0 ps1
+        rred (Eassignop op (Eloc (Ltmp b) ty1) (Eval (v2,vt2) ty2) tyres ty1) te m E0
+             (Eassign (Eloc (Ltmp b) ty1)
+                      (Ebinop op (Eval (v1,vt1') ty1) (Eval (v2,vt2) ty2) tyres) ty1) te m ps0 ps1
     | red_assignop_ifun: forall op b pt ty1 v2 vt2 ty2 tyres te m ps,
-        rred pct (Eassignop op (Eloc (Lifun b pt) ty1) (Eval (v2,vt2) ty2) tyres ty1) te m E0
-             pct (Eassign (Eloc (Lifun b pt) ty1)
-                          (Ebinop op (Eval (Vfptr b,pt) ty1) (Eval (v2,vt2) ty2) tyres) ty1) te m ps ps
+        rred (Eassignop op (Eloc (Lifun b pt) ty1) (Eval (v2,vt2) ty2) tyres ty1) te m E0
+             (Eassign (Eloc (Lifun b pt) ty1)
+                      (Ebinop op (Eval (Vfptr b,pt) ty1) (Eval (v2,vt2) ty2) tyres) ty1) te m ps ps
     | red_assignop_efun: forall op ef tyargs tyres cc pt ty1 v2 vt2 ty2 ty te m ps,
-        rred pct (Eassignop op (Eloc (Lefun ef tyargs tyres cc pt) ty1)
+        rred (Eassignop op (Eloc (Lefun ef tyargs tyres cc pt) ty1)
                             (Eval (v2,vt2) ty2) ty ty1) te m E0
-             pct (Eassign (Eloc (Lefun ef tyargs tyres cc pt) ty1)
-                          (Ebinop op (Eval (Vefptr ef tyargs tyres cc,pt) ty1)
-                                  (Eval (v2,vt2) ty2) ty) ty1) te m ps ps
+             (Eassign (Eloc (Lefun ef tyargs tyres cc pt) ty1)
+                      (Ebinop op (Eval (Vefptr ef tyargs tyres cc,pt) ty1)
+                              (Eval (v2,vt2) ty2) ty) ty1) te m ps ps
     | red_postincr_mem: forall id ofs pt ty bf te m t v vts vt'' lts op ps0 ps1 ps2,
         deref_loc ty m ofs pt bf t <<ps0>> (Success (v, vts, lts)) <<ps1>> ->
         op = match id with Incr => Oadd | Decr => Osub end ->
-        (vt <- CoalesceT l vts;;
-         vt' <- LoadT l pct pt vt lts;;
-         AccessT l pct vt') ps1 = (Success vt'',ps2) ->
-        rred pct (Epostincr id (Eloc (Lmem ofs pt bf) ty) ty) te m t
-             pct (Ecomma (Eassign (Eloc (Lmem ofs pt bf) ty)
-                                  (Ebinop op (Eval (v,vt'') ty)
-                                          (Econst (Vint Int.one) type_int32s)
-                                          (incrdecr_type ty))
-                                  ty)
-                         (Eval (v,vt'') ty) ty) te m ps0 ps2
+        rred (Epostincr id (Eloc (Lmem ofs pt bf) ty) ty) te m t
+             (Ecomma (Eassign (Eloc (Lmem ofs pt bf) ty)
+                              (Ebinop op (Eval (v,vt'') ty)
+                                      (Econst (Vint Int.one) type_int32s)
+                                      (incrdecr_type ty))
+                              ty)
+                     (Eval (v,vt'') ty) ty) te m ps0 ps2
     | red_postincr_tmp: forall id b ty te m v vt vt' op ps0 ps1,
         te!b = Some (v,vt) ->
         op = match id with Incr => Oadd | Decr => Osub end ->
-        AccessT l pct vt ps0 = (Success vt', ps1) ->
-        rred pct (Epostincr id (Eloc (Ltmp b) ty) ty) te m E0
-             pct (Ecomma (Eassign (Eloc (Ltmp b) ty)
-                                  (Ebinop op (Eval (v,vt') ty)
-                                          (Econst (Vint Int.one) type_int32s)
-                                          (incrdecr_type ty))
-                                  ty)
-                         (Eval (v,vt') ty) ty) te m ps0 ps1
+        rred (Epostincr id (Eloc (Ltmp b) ty) ty) te m E0
+             (Ecomma (Eassign (Eloc (Ltmp b) ty)
+                              (Ebinop op (Eval (v,vt') ty)
+                                      (Econst (Vint Int.one) type_int32s)
+                                      (incrdecr_type ty))
+                              ty)
+                     (Eval (v,vt') ty) ty) te m ps0 ps1
     | red_postincr_ifun: forall id b pt ty te m op ps,
         op = match id with Incr => Oadd | Decr => Osub end ->
-        rred pct (Epostincr id (Eloc (Lifun b pt) ty) ty) te m E0
-             pct (Ecomma (Eassign (Eloc (Lifun b pt) ty)
-                                  (Ebinop op (Eval (Vfptr b, pt) ty)
-                                          (Econst (Vint Int.one) type_int32s)
-                                          (incrdecr_type ty))
-                                  ty)
-                         (Eval (Vfptr b,pt) ty) ty) te m ps ps
+        rred (Epostincr id (Eloc (Lifun b pt) ty) ty) te m E0
+             (Ecomma (Eassign (Eloc (Lifun b pt) ty)
+                              (Ebinop op (Eval (Vfptr b, pt) ty)
+                                      (Econst (Vint Int.one) type_int32s)
+                                      (incrdecr_type ty))
+                              ty)
+                     (Eval (Vfptr b,pt) ty) ty) te m ps ps
     | red_postincr_efun: forall id ef tyargs tyres cc pt ty te m op ps,
         op = match id with Incr => Oadd | Decr => Osub end ->
-        rred pct (Epostincr id (Eloc (Lefun ef tyargs tyres cc pt) ty) ty) te m E0
-             pct (Ecomma (Eassign (Eloc (Lefun ef tyargs tyres cc pt) ty)
-                                  (Ebinop op (Eval (Vefptr ef tyargs tyres cc, pt) ty)
-                                          (Econst (Vint Int.one) type_int32s)
-                                          (incrdecr_type ty))
-                                  ty)
-                         (Eval (Vefptr ef tyargs tyres cc,pt) ty) ty) te m ps ps
+        rred (Epostincr id (Eloc (Lefun ef tyargs tyres cc pt) ty) ty) te m E0
+             (Ecomma (Eassign (Eloc (Lefun ef tyargs tyres cc pt) ty)
+                              (Ebinop op (Eval (Vefptr ef tyargs tyres cc, pt) ty)
+                                      (Econst (Vint Int.one) type_int32s)
+                                      (incrdecr_type ty))
+                              ty)
+                     (Eval (Vefptr ef tyargs tyres cc,pt) ty) ty) te m ps ps
     | red_comma: forall v ty1 r2 ty te m ps,
         typeof r2 = ty ->
-        rred pct (Ecomma (Eval v ty1) r2 ty) te m E0
-             pct r2 te m ps ps
-    | red_paren: forall v1 vt1 ty1 ty2 ty te m v pct' vt' ps0 ps1,
-        sem_cast v1 ty1 ty2 m = Some v ->
-        ExprJoinT l pct vt1 ps0 = (Success (pct', vt'),ps1) ->
-        rred pct (Eparen (Eval (v1,vt1) ty1) ty2 ty) te m E0
-             pct' (Eval (v,vt') ty) te m ps0 ps1.
+        rred (Ecomma (Eval v ty1) r2 ty) te m E0 r2 te m ps ps
+    | red_paren: forall v1 vt1 ty1 ty2 ty te m v vt' ps0 ps1,
+        sem_cast v1 ty1 ty2 (Lcl CMP) = Some v ->
+        rred (Eparen (Eval (v1,vt1) ty1) ty2 ty) te m E0
+             (Eval (v,vt') ty) te m ps0 ps1.
 
     (** Failstops for r-values *)
-    Inductive rfailred (pct:control_tag) :
+    Inductive rfailred :
       expr -> tenv -> mem -> trace -> FailureClass -> pstate -> pstate -> Prop :=
-    | failred_const:
-      forall v ty te m failure ps ps',
-        ConstT l pct ps = (Fail failure, ps') ->
-        rfailred pct (Econst v ty) te m E0 failure ps ps'
     | failred_rvalof_mem0:
       forall ofs pt bf ty te m tr failure ps0 ps1,
         deref_loc ty m ofs pt bf tr <<ps0>> (Fail failure) <<ps1>> ->
-        rfailred pct (Evalof (Eloc (Lmem ofs pt bf) ty) ty) te m tr failure ps0 ps1
-    | failred_rvalof_mem1:
-      forall ofs pt lts bf ty te m tr v vts failure ps0 ps1 ps2,
-        deref_loc ty m ofs pt bf tr <<ps0>> (Success (v, vts, lts)) <<ps1>> ->
-        (vt <- CoalesceT l vts;;
-        vt' <- LoadT l pct pt vt lts;;
-        AccessT l pct vt') ps1 = (Fail failure, ps2) ->
-        rfailred pct (Evalof (Eloc (Lmem ofs pt bf) ty) ty) te m tr failure ps0 ps2
-    | failred_rvalof_tmp:
-      forall b ty te m v vt failure ps0 ps1,
-        te!b = Some (v,vt) ->
-        AccessT l pct vt ps0 = (Fail failure,ps1) ->
-        rfailred pct (Evalof (Eloc (Ltmp b) ty) ty) te m E0 failure ps0 ps1
-    | failred_unop:
-      forall op v1 vt1 ty1 ty te m v failure ps0 ps1,
-        sem_unary_operation op v1 ty1 m = Some v ->
-        UnopT l op pct vt1 ps0 = (Fail failure,ps1) ->
-        rfailred pct (Eunop op (Eval (v1,vt1) ty1) ty) te m E0 failure ps0 ps1
-    | failred_binop:
-      forall op v1 vt1 ty1 v2 vt2 ty2 ty te m v failure ps0 ps1,
-        sem_binary_operation ce op v1 ty1 v2 ty2 m = Some v ->
-        BinopT l op pct vt1 vt2 ps0 = (Fail failure,ps1) ->
-        rfailred pct (Ebinop op (Eval (v1,vt1) ty1) (Eval (v2,vt2) ty2) ty) te m E0 failure ps0 ps1
-    | failred_seqand:
-      forall v1 vt1 ty1 r2 ty b te m failure ps0 ps1,
-        bool_val v1 ty1 m = Some b ->
-        ExprSplitT l pct vt1 ps0 = (Fail failure,ps1) ->
-        rfailred pct (Eseqand (Eval (v1,vt1) ty1) r2 ty) te m E0 failure ps0 ps1
-    | failred_seqor:
-      forall v1 vt1 ty1 r2 ty b te m failure ps0 ps1,
-        bool_val v1 ty1 m = Some b ->
-        ExprSplitT l pct vt1 ps0 = (Fail failure,ps1) ->
-        rfailred pct (Eseqor (Eval (v1,vt1) ty1) r2 ty) te m E0 failure ps0 ps1
-    | failred_condition:
-      forall v1 vt1 ty1 r1 r2 ty b te m failure ps0 ps1,
-        bool_val v1 ty1 m = Some b ->
-        ExprSplitT l pct vt1 ps0 = (Fail failure,ps1) ->
-        rfailred pct (Econdition (Eval (v1,vt1) ty1) r1 r2 ty) te m E0 failure ps0 ps1
-    | failred_sizeof:
-      forall ty1 ty te m failure ps0 ps1,
-        ConstT l pct ps0 = (Fail failure,ps1) ->
-        rfailred pct (Esizeof ty1 ty) te m E0 failure ps0 ps1
-    | failred_alignof:
-      forall ty1 ty te m failure ps0 ps1,
-        ConstT l pct ps0 = (Fail failure,ps1) ->
-        rfailred pct (Ealignof ty1 ty) te m E0 failure ps0 ps1
+        rfailred (Evalof (Eloc (Lmem ofs pt bf) ty) ty) te m tr failure ps0 ps1
     | failred_assign_mem0:
       forall ofs ty1 pt bf v2 vt2 ty2 te m t1 v' failure ps0 ps1,
-        sem_cast v2 ty2 ty1 m = Some v' ->
+        sem_cast v2 ty2 ty1 (Lcl CMP) = Some v' ->
         deref_loc ty1 m ofs pt bf t1 <<ps0>> (Fail failure) <<ps1>> ->
-        rfailred pct (Eassign (Eloc (Lmem ofs pt bf) ty1)
+        rfailred (Eassign (Eloc (Lmem ofs pt bf) ty1)
                               (Eval (v2, vt2) ty2) ty1) te m t1 failure ps0 ps1
-    | failred_assign_mem1:
-      forall ofs ty1 pt bf v1 vts v2 vt2 ty2 te m t1 v' lts failure ps0 ps1 ps2,
-        sem_cast v2 ty2 ty1 m = Some v' ->
-        deref_loc ty1 m ofs pt bf t1 <<ps0>> (Success (v1, vts, lts)) <<ps1>> ->
-        ('(pct',vt') <- AssignT l pct (EffectiveT l vts) vt2;;
-         StoreT l pct' pt vt' lts) ps1 = (Fail failure,ps2) ->
-        rfailred pct (Eassign (Eloc (Lmem ofs pt bf) ty1) (Eval (v2, vt2) ty2) ty1) te m t1 failure ps0 ps1
     | failred_assign_mem2:
-      forall ofs ty1 pt bf v1 vts v2 vt2 ty2 te m t1 v' lts pct'' vt'' lts' t2 failure ps0 ps1 ps2 ps3,
-        sem_cast v2 ty2 ty1 m = Some v' ->
+      forall ofs ty1 pt bf v1 vts v2 vt2 ty2 te m t1 v' lts vt'' lts' t2 failure ps0 ps1 ps2 ps3,
+        sem_cast v2 ty2 ty1 (Lcl CMP) = Some v' ->
         deref_loc ty1 m ofs pt bf t1 <<ps0>> (Success (v1, vts, lts)) <<ps1>> ->
-        ('(pct',vt') <- AssignT l pct (EffectiveT l vts) vt2;;
-         StoreT l pct' pt vt' lts) ps1 = (Success (pct'',vt'',lts'),ps2) ->
         assign_loc ty1 m ofs pt lts' bf (v',vt'') t2 <<ps2>> (Fail failure) <<ps3>> ->
-        rfailred pct (Eassign (Eloc (Lmem ofs pt bf) ty1) (Eval (v2, vt2) ty2) ty1) te m (t1++t2) failure ps0 ps3
-    | failred_assign_tmp:
-      forall b ty1 v1 vt1 v2 vt2 ty2 te m v failure ps0 ps1,
-        te!b = Some (v1,vt1) ->
-        sem_cast v2 ty2 ty1 m = Some v ->
-        AssignT l pct vt1 vt2 ps0 = (Fail failure,ps1) ->
-        rfailred pct (Eassign (Eloc (Ltmp b) ty1) (Eval (v2, vt2) ty2) ty1) te m E0 failure ps0 ps1
+        rfailred (Eassign (Eloc (Lmem ofs pt bf) ty1)
+                          (Eval (v2, vt2) ty2) ty1) te m (t1++t2) failure ps0 ps3
     | failred_assignop_mem0:
       forall op ofs pt ty1 bf v2 vt2 ty2 tyres te m t1 failure ps0 ps1,
         deref_loc ty1 m ofs pt bf t1 <<ps0>> (Fail failure) <<ps1>> ->
-        rfailred pct (Eassignop op (Eloc (Lmem ofs pt bf) ty1)
+        rfailred (Eassignop op (Eloc (Lmem ofs pt bf) ty1)
                                 (Eval (v2,vt2) ty2) tyres ty1) te m t1 failure ps0 ps1
-    | failred_assignop_mem1:
-      forall op ofs pt ty1 bf v2 vt2 ty2 tyres te m t1 v1 vts lts failure ps0 ps1 ps2,
-        deref_loc ty1 m ofs pt bf t1 <<ps0>> (Success (v1,vts, lts)) <<ps1>> ->
-        (vt1 <- CoalesceT l vts;;
-         vt1' <- LoadT l pct pt vt1 lts;;
-         AccessT l pct vt1') ps1 = (Fail failure,ps2) ->
-        rfailred pct (Eassignop op (Eloc (Lmem ofs pt bf) ty1)
-                                (Eval (v2,vt2) ty2) tyres ty1) te m t1 failure ps0 ps2
-    | failred_assignop_tmp:
-      forall op b ty1 v2 vt2 ty2 tyres te m v1 vt1 failure ps0 ps1,
-        te!b = Some (v1,vt1) ->
-        AccessT l pct vt1 ps0 = (Fail failure,ps1) ->
-        rfailred pct (Eassignop op (Eloc (Ltmp b) ty1) (Eval (v2,vt2) ty2) tyres ty1) te m E0 failure ps0 ps1
     | failred_postincr_mem0:
       forall id ofs pt ty bf te m tr failure ps0 ps1,
         deref_loc ty m ofs pt bf tr <<ps0>> (Fail failure) <<ps1>> ->
-        rfailred pct (Epostincr id (Eloc (Lmem ofs pt bf) ty) ty) te m tr failure ps0 ps1
-    | failred_postincr_mem1:
-      forall id ofs pt ty bf te m tr v vts lts failure ps0 ps1 ps2,
-        deref_loc ty m ofs pt bf tr <<ps0>> (Success (v,vts, lts)) <<ps1>> ->
-        (vt <- CoalesceT l vts;;
-         vt' <- LoadT l pct pt vt lts;;
-         AccessT l pct vt') ps1 = (Fail failure,ps2) ->
-        rfailred pct (Epostincr id (Eloc (Lmem ofs pt bf) ty) ty) te m tr failure ps0 ps2
-    | failred_postincr_tmp:
-      forall id b ty te m v vt failure ps0 ps1,
-        te!b = Some (v,vt) ->
-        AccessT l pct vt ps0 = (Fail failure, ps1) ->
-        rfailred pct (Epostincr id (Eloc (Ltmp b) ty) ty) te m E0 failure ps0 ps1
-    | failred_paren:
-      forall v1 vt1 ty1 ty2 ty te m v failure ps0 ps1,
-        sem_cast v1 ty1 ty2 m = Some v ->
-        ExprJoinT l pct vt1 ps0 = (Fail failure,ps1) ->
-        rfailred pct (Eparen (Eval (v1,vt1) ty1) ty2 ty) te m E0 failure ps0 ps1
-    | failred_cast_int_int:
-      forall ty v1 vt1 ty1 te m v failure ps0 ps1,
-        (forall ty' attr, ty1 <> Tpointer ty' attr) ->
-        (forall ty' attr, ty <> Tpointer ty' attr) ->
-        sem_cast v1 ty1 ty m = Some v ->
-        IICastT l pct vt1 ty ps0 = (Fail failure,ps1) -> 
-        rfailred pct (Ecast (Eval (v1,vt1) ty1) ty) te m E0 failure ps0 ps1
-    | failred_cast_int_ptr:
-      forall ty v1 vt1 ty1 te m v ofs tr v2 vt2 lts ty' attr failure ps0 ps1 ps2,
-        (forall ty' attr, ty1 <> Tpointer ty' attr) ->
-        ty = Tpointer ty' attr ->
-        sem_cast v1 ty1 ty m = Some v ->
-        v = Vptr ofs ->
-        deref_loc ty m ofs vt1 Full tr <<ps0>> (Success ((v2,vt2), lts)) <<ps1>> ->
-        IPCastT l pct vt1 (Some lts) ty ps0 = (Fail failure,ps2) ->
-        rfailred pct (Ecast (Eval (v1,vt1) ty1) ty) te m tr failure ps0 ps2
-    | failred_cast_ptr_int:
-      forall ty v1 vt1 ty1 te m v ofs tr v2 vt2 lts ty' attr failure ps0 ps1 ps2,
-        ty1 = Tpointer ty' attr ->
-        (forall ty' attr, ty <> Tpointer ty' attr) ->
-        sem_cast v1 ty1 ty m = Some v ->
-        v1 = Vptr ofs ->
-        deref_loc ty1 m ofs vt1 Full tr <<ps0>> (Success ((v2,vt2), lts)) <<ps1>> ->
-        PICastT l pct vt1 (Some lts) ty ps1 = (Fail failure, ps2) ->
-        rfailred pct (Ecast (Eval (v1,vt1) ty1) ty) te m tr failure ps0 ps2
-    | failred_cast_ptr_ptr:
-      forall ty v1 vt1 ty1 te m v ofs ofs1 tr tr1 v2 vt2 v3 vt3 lts lts1 ty1' attr1 ty' attr2 failure ps0 ps1 ps2 ps3,
-        ty1 = Tpointer ty1' attr1 ->
-        ty = Tpointer ty' attr2 ->
-        sem_cast v1 ty1 ty m = Some v ->
-        v1 = Vptr ofs1 ->
-        v = Vptr ofs ->
-        deref_loc ty1 m ofs1 vt1 Full tr1 <<ps0>> (Success ((v2,vt2), lts1)) <<ps1>> ->
-        deref_loc ty m ofs vt1 Full tr <<ps1>> (Success ((v3,vt3), lts)) <<ps2>> ->
-        PPCastT l pct vt1 (Some lts1) (Some lts) ty ps2 = (Fail failure,ps3) ->
-        rfailred pct (Ecast (Eval (v1,vt1) ty1) ty) te m (tr1 ++ tr) failure ps0 ps3
-
+        rfailred (Epostincr id (Eloc (Lmem ofs pt bf) ty) ty) te m tr failure ps0 ps1
     | red_call_internal_fail: forall ty te m b fd vft tyf tyargs tyres cconv el failure ps0 ps1,
         Genv.find_funct ge (Vfptr b) = Some fd ->
         type_of_fundef fd = Tfunction tyargs tyres cconv ->
         classify_fun tyf = fun_case_f tyargs tyres cconv ->
-        cast_arguments l pct vft m el tyargs <<ps0>> (Fail failure) <<ps1>> ->
-        rfailred pct (Ecall (Eval (Vfptr b,vft) tyf) el ty) te m E0 failure ps0 ps1
+        cast_arguments l CMP vft m el tyargs <<ps0>> (Fail failure) <<ps1>> ->
+        rfailred (Ecall (Eval (Vfptr b,vft) tyf) el ty) te m E0 failure ps0 ps1
     | red_call_external_fail: forall vft tyf te m tyargs tyres cconv el ty ef failure ps0 ps1,
-        cast_arguments l pct vft m el tyargs <<ps0>> (Fail failure) <<ps1>> ->
-        rfailred pct (Ecall (Eval (Vefptr ef tyargs tyres cconv,vft) tyf) el ty) te m E0
+        cast_arguments l CMP vft m el tyargs <<ps0>> (Fail failure) <<ps1>> ->
+        rfailred (Ecall (Eval (Vefptr ef tyargs tyres cconv,vft) tyf) el ty) te m E0
                  failure ps0 ps1
     .
 
-    Inductive callred: control_tag -> expr -> mem -> fundef ->
-                       val_tag -> list atom -> type -> control_tag ->
+    Inductive callred: expr -> mem -> fundef ->
+                       val_tag -> list atom -> type ->
                        pstate -> pstate -> Prop :=
-    | red_call_internal: forall pct pct' b vft tyf m tyargs tyres cconv el ty fd vargs ps0 ps1,
+    | red_call_internal: forall b vft tyf m tyargs tyres cconv el ty fd vargs ps0 ps1,
         Genv.find_funct ge (Vfptr b) = Some fd ->
         type_of_fundef fd = Tfunction tyargs tyres cconv ->
         classify_fun tyf = fun_case_f tyargs tyres cconv ->
-        cast_arguments l pct vft m el tyargs <<ps0>> (Success (pct',vargs)) <<ps1>> ->
-        callred pct (Ecall (Eval (Vfptr b,vft) tyf) el ty) m
-                fd vft vargs ty pct' ps0 ps1
-    | red_call_external: forall pct pct' vft tyf m tyargs tyres cconv el ty ef vargs ps0 ps1,
-        cast_arguments l pct vft m el tyargs <<ps0>> (Success (pct',vargs)) <<ps1>> ->
-        callred pct (Ecall (Eval (Vefptr ef tyargs tyres cconv,vft) tyf) el ty)
-                m (External ef tyargs ty cconv) vft vargs ty pct' ps0 ps1.
+        cast_arguments l CMP vft m el tyargs <<ps0>> (Success (vargs)) <<ps1>> ->
+        callred (Ecall (Eval (Vfptr b,vft) tyf) el ty) m
+                fd vft vargs ty ps0 ps1
+    | red_call_external: forall vft tyf m tyargs tyres cconv el ty ef vargs ps0 ps1,
+        cast_arguments l CMP vft m el tyargs <<ps0>> (Success vargs) <<ps1>> ->
+        callred (Ecall (Eval (Vefptr ef tyargs tyres cconv,vft) tyf) el ty)
+                m (External ef tyargs ty cconv) vft vargs ty ps0 ps1.
  
     (** Reduction contexts.  In accordance with C's nondeterministic semantics,
         we allow reduction both to the left and to the right of a binary operator.
@@ -917,33 +755,31 @@ Module CompartmentCsem (Scheme: CompScheme) (A: AllocatorAxioms SemiconcretePoin
     | ctx_list_tail: forall k C e1,
         contextlist k C -> contextlist k (fun x => Econs e1 (C x)).
 
-    Inductive imm_safe: kind -> expr -> control_tag -> tenv -> mem -> Prop :=
-  | imm_safe_val: forall v ty pct te m,
-      imm_safe RV (Eval v ty) pct te m
-  | imm_safe_loc: forall lk ty pct te m,
-      imm_safe LV (Eloc lk ty) pct te m
-  | imm_safe_lred: forall pct to C e te m e' te' m' s s',
-      lred e pct te m e' te' m' s s' ->
+    Inductive imm_safe: kind -> expr -> tenv -> mem -> Prop :=
+  | imm_safe_val: forall v ty te m,
+      imm_safe RV (Eval v ty) te m
+  | imm_safe_loc: forall lk ty te m,
+      imm_safe LV (Eloc lk ty) te m
+  | imm_safe_lred: forall to C e te m e' te' m' s s',
+      lred e te m e' te' m' s s' ->
       context LV to C ->
-      imm_safe to (C e) pct te m
-  | imm_safe_rred: forall pct pct' to C e te m t e' te' m' s s',
-      rred pct e te m t pct' e' te' m' s s' ->
+      imm_safe to (C e) te m
+  | imm_safe_rred: forall to C e te m t e' te' m' s s',
+      rred e te m t e' te' m' s s' ->
       context RV to C ->
-      imm_safe to (C e) pct te m
-  | imm_safe_rfailred: forall pct to C e te m tr failure s s',
-      rfailred pct e te m tr failure s s' ->
+      imm_safe to (C e) te m
+  | imm_safe_rfailred: forall to C e te m tr failure s s',
+      rfailred e te m tr failure s s' ->
       context RV to C ->
-      imm_safe to (C e) pct te m
-  | imm_safe_callred: forall pct to C e te m fd fpt args ty pct' s s',
-      callred pct e m fd fpt args ty pct' s s' ->
+      imm_safe to (C e) te m
+  | imm_safe_callred: forall to C e te m fd fpt args ty s s',
+      callred e m fd fpt args ty s s' ->
       context RV to C ->
-      imm_safe to (C e) pct te m.
-
-
+      imm_safe to (C e) te m.
  
     Definition not_stuck (e: expr) (te: tenv) (m: mem) : Prop :=
-      forall k C e' pct,
-        context k RV C -> e = C e' -> imm_safe k e' pct te m.
+      forall k C e' ,
+        context k RV C -> e = C e' -> imm_safe k e' te m.
 
 
 
@@ -968,7 +804,6 @@ Inductive cont: Type :=
          env ->                (**r local env of calling function *)
          tenv ->               (**r temp env of calling function *)
          Cabs.loc ->           (**r location before call *)
-         control_tag ->                (**r PC tag before call *)
          (expr -> expr) ->     (**r context of the call *)
          type ->               (**r type of call expression *)
          cont -> cont.
@@ -989,13 +824,13 @@ Fixpoint call_cont (k: cont) : cont :=
   | Kswitch1 ls k => call_cont k
   | Kswitch2 k => call_cont k
   | Kreturn k => call_cont k
-  | Kcall _ _ _ _ _ _ _ _ => k
+  | Kcall _ _ _ _ _ _ _ => k
   end.
 
 Definition is_call_cont (k: cont) : Prop :=
   match k with
   | Kstop => True
-  | Kcall _ _ _ _ _ _ _ _ => True
+  | Kcall _ _ _ _ _ _ _ => True
   | _ => False
   end.
 
@@ -1025,7 +860,7 @@ Inductive state': Type :=
     (fd: fundef)                      (* callee that has just been entered *)
     (l: Cabs.loc)
     (ps: pstate)
-    (C: Comp)
+    (C: Comp)                         (* Compartment making the call *)
     (bg: block_generator)
     (args: list atom)
     (k: cont)
@@ -1034,7 +869,7 @@ Inductive state': Type :=
     (fd: fundef)                      (* callee that is now returning *)
     (l: Cabs.loc)
     (ps: pstate)
-    (C: Comp)
+    (C: Comp)                         (* Compartment now returning *)
     (bg: block_generator)
     (res: atom)
     (k: cont)
@@ -1093,23 +928,23 @@ with find_label_ls (lbl: label) (sl: labeled_statements) (k: cont)
 
 Inductive estep: state -> trace -> state -> Prop :=
 | step_lred: forall C f l CMP bg a k e te a' m te' m' ps ps',
-    lred e l a tt te m a' te' m' ps ps' ->
+    lred e a te m a' te' m' ps ps' ->
     context LV RV C ->
     estep (ExprState f l ps CMP bg (C a) k e te m)
           E0 (ExprState f l ps' CMP bg (C a') k e te' m')
 | step_rred: forall C f l CMP bg a k e te m tr a' te' m' ps ps',
-    rred l tt a te m tr tt a' te' m' ps ps'->
+    rred CMP a te m tr a' te' m' ps ps'->
     context RV RV C ->
     estep (ExprState f l ps CMP bg (C a) k e te m)
           tr (ExprState f l ps' CMP bg (C a') k e te' m')
-| step_call: forall C f l CMP bg pct pct' fpt a k e te m fd vargs ty ps ps',
-    callred l pct a m fd fpt vargs ty pct' ps ps' ->
+| step_call: forall C f l CMP bg fpt a k e te m fd vargs ty ps ps',
+    callred l CMP a m fd fpt vargs ty ps ps' ->
     context RV RV C ->
     estep (ExprState f l ps CMP bg (C a) k e te m)
-          E0 (Callstate fd l ps' CMP bg vargs (Kcall f e te l pct C ty k) m)
-| step_stuck: forall C f l CMP bg pct a k e te m K ps,
-    context K RV C -> ~(imm_safe e l K a pct te m) ->
-    estep (ExprState f l ps bg CMP (C a) k e te m)
+          E0 (Callstate fd l ps' CMP bg vargs (Kcall f e te l C ty k) m)
+| step_stuck: forall C f l CMP bg a k e te m K ps,
+    context K RV C -> ~(imm_safe e l CMP K a te m) ->
+    estep (ExprState f l ps CMP bg (C a) k e te m)
           E0 Stuckstate
 | step_rfail: forall C f l CMP bg pct a k e te m tr failure ps ps',
     rfailred l pct a te m tr failure ps ps' ->
@@ -1235,12 +1070,12 @@ Inductive sstep: state -> trace -> state -> Prop :=
     sstep (State f ps CMP bg (Sreturn (Some x) l) k e te m)
           E0 (ExprState f l ps CMP bg x (Kreturn k) e te m)
 | step_return_2:  forall f ps CMP bg l v vt ty k e te m v' m',
-    sem_cast v ty f.(fn_return) m = Some v' ->
+    sem_cast v ty f.(fn_return) (Lcl CMP) = Some v' ->
     do_free_variables l CMP tt m (variables_of_env e) = ret (tt, m') ->
     sstep (ExprState f l ps CMP bg (Eval (v,vt) ty) (Kreturn k) e te m)
           E0 (Returnstate (Internal f) l ps CMP bg (v',vt) (call_cont k) m')
 | step_return_fail0:  forall f ps CMP bg pct l v vt ty k e te m v' failure,
-    sem_cast v ty f.(fn_return) m = Some v' ->
+    sem_cast v ty f.(fn_return) (Lcl CMP) = Some v' ->
     do_free_variables l CMP pct m (variables_of_env e) = raise failure ->
     sstep (ExprState f l ps CMP bg (Eval (v,vt) ty) (Kreturn k) e te m)
           E0 (Failstop failure (snd ps))
@@ -1293,12 +1128,12 @@ Inductive sstep: state -> trace -> state -> Prop :=
     sstep (Callstate (Internal f) l ps CMP bg vargs k m)
           E0 (Failstop failure (snd ps''))
 
-| step_external_function: forall l ef ps CMP bg pct vft pct' targs tres cc vargs k m vres t m',
-    external_call l ef (Lcl CMP) ge vargs pct vft m t (ret (vres, pct', m')) ->
+| step_external_function: forall l ef ps CMP bg pct' targs tres cc vargs k m vres t m',
+    external_call l ef (Lcl CMP) ge vargs tt tt m t (ret (vres, pct', m')) ->
     sstep (Callstate (External ef targs tres cc) l ps CMP bg vargs k m)
           t (Returnstate (External ef targs tres cc) l ps CMP bg vres k m')
-| step_external_function_fail0: forall l ef ps CMP bg pct vft targs tres cc vargs k m t failure,
-    external_call l ef (Lcl CMP) ge vargs pct vft m t (raise failure) ->
+| step_external_function_fail0: forall l ef ps CMP bg targs tres cc vargs k m t failure,
+    external_call l ef (Lcl CMP) ge vargs tt tt m t (raise failure) ->
     sstep (Callstate (External ef targs tres cc) l ps CMP bg vargs k m)
           t (Failstop failure (snd ps))
 | step_external_function_fail1: forall l ef ps CMP bg pct vft targs tres cc vargs k m t failure,
@@ -1306,8 +1141,8 @@ Inductive sstep: state -> trace -> state -> Prop :=
     sstep (Callstate (External ef targs tres cc) l ps CMP bg vargs k m)
           t (Failstop failure (snd ps))
 
-| step_returnstate: forall l v vt vt' f fd ps CMP bg oldloc oldpct  C ty k e te m,
-    sstep (Returnstate fd l ps CMP bg (v,vt) (Kcall f e te oldloc oldpct C ty k) m)
+| step_returnstate: forall l v vt vt' f fd ps CMP bg oldloc C ty k e te m,
+    sstep (Returnstate fd l ps CMP bg (v,vt) (Kcall f e te oldloc C ty k) m)
           E0 (ExprState f oldloc ps CMP bg (C (Eval (v,vt') ty)) k e te m)
 .
 
